cleanup/Example.v
@@ -13,7 +13,7 @@ From Coq.Arith Require Import Arith EqNat.
 Open Scope string_scope.
 Open Scope list_scope.
 From Taxiway Require Import Types.
-From Taxiway Require Import Implementation.
+From Taxiway Require Import Find_path.
 
 (* ============ vertex ============*)
 
