cleanup/Extraction.v
@@ -3,7 +3,7 @@
     In default, this file won't be compiled use "make"
 *)
 
-From Taxiway Require Export Implementation.
+From Taxiway Require Export Find_path.
 
 Require Coq.extraction.Extraction.
 Extraction "find_path.ml" find_path.
